KripkeMetatheory.v
@@ -1,4 +1,4 @@
-Require Import ssreflect stdpp.propset.
+Require Import ssreflect stdpp.propset stdpp.relations.
 Require Import Classical.
 
 Require Import Flowers.Syntax Flowers.KripkeSemantics Flowers.Utils.
@@ -9,9 +9,49 @@ Context (Σ : sig).
 
 Section Soundness.
 
-Theorem soundness (ϕ : wfflower) :
-  sprov ϕ -> ∀ A (K : KModel A), ∅ ⊨ ϕ.
+Context A (K : KModel A).
+
+Lemma local_soundness (Φ Ψ : wfbouquet) :
+  Φ ⇀ Ψ -> Φ ⫤⊨ Ψ.
+Admitted.
+
+Lemma grounding : ∀ (X : wfctx) (Φ Ψ : wfbouquet),
+  Φ ⫤⊨ Ψ -> btot (X ⋖ Φ ⇂ wf_fill X Φ) ⫤⊨ btot (X ⋖ Ψ ⇂ wf_fill X Ψ).
+Admitted.
+
+Lemma pgrounding : ∀ (P : wfpctx) (Φ Ψ : wfbouquet),
+  Φ ⊨ Ψ -> btot (P ⋖ Φ ⇂ wf_fill P Φ) ⊨ btot (P ⋖ Ψ ⇂ wf_fill P Ψ).
+Admitted.
+
+Lemma in_bouquet : ∀ (Φ : bouquet) (H H' : wf Φ) ϕ,
+  ϕ ∈ btot (Φ ⇂ H) <-> ϕ ∈ btot (Φ ⇂ H').
 Proof.
+  done.
+Qed.
+
+Lemma entails_refl (Φ : bouquet) (H H' : wf Φ) :
+  btot (Φ ⇂ H) ⊨ btot (Φ ⇂ H').
+Proof.
+  intros ?? Hf ϕ. by apply (Hf ϕ).
+Qed.
+
+Lemma eqentails_refl (Φ : bouquet) (H H' : wf Φ) :
+  btot (Φ ⇂ H) ⫤⊨ btot (Φ ⇂ H').
+Proof.
+  split; by apply entails_refl.
+Qed.
+
+Lemma wf_cstep {Φ Ψ : bouquet} :
+  Φ ≈> Ψ -> wf Φ -> wf Ψ.
+Admitted.
+
+Theorem soundness : ∀ (Φ Ψ : wfbouquet),
+  Φ ≈>* Ψ -> Φ ⫤⊨ Ψ.
+Proof.
+  move => [Φ HΦ] [Ψ HΨ]. do 2 rewrite [bfgt _]/=.
+  induction 1 as [Φ |Φ1 Φ2 Φ3 Hstep H IH].
+  * by apply eqentails_refl.
+  * rewrite -(IH (wf_cstep Hstep HΦ) HΨ). admit.
 Admitted.
 
 End Soundness.
@@ -63,5 +103,4 @@ Theorem structural_admissibility (ϕ : wfflower) :
   sprov ϕ -> prov ϕ.
 Proof.
   intros. apply completeness. intros.
-  by apply soundness.
-Qed.
+Admitted.
